IrisCore/iPropShallow.thy
@@ -32,9 +32,6 @@ ML \<open>
   }
 
   (* Names *)
-  val iPropN = Binding.name "iProp"
-  val preN = Binding.name "pre"
-  val pre_ipropN = Binding.name "pre_iprop"
   val resFN = Binding.name "resF"
   val invN = Binding.name "inv"
   val resN = Binding.name "res"
@@ -45,6 +42,7 @@ ML \<open>
   val mapN = "map_res"
 
   (* Types *)
+  val pre_ipropT = \<^typ>\<open>pre_iprop\<close>
   val gnameT = \<^typ>\<open>gname\<close>
   fun mk_opt T = Type (\<^type_name>\<open>option\<close>, [T])
   fun mk_res_mapT res = gnameT --> mk_opt res (* This might need to be (gname,res) fmap *)
@@ -136,12 +134,6 @@ ML \<open>
     end
 
   (* Setup functions *)
-  val mk_pre_iprop = Typedecl.typedecl_global {final=false} (pre_ipropN,[],NoSyn)
-
-  fun mk_axioms preT propT = 
-    [(iPropN,SOME (preT --> propT),NoSyn),(preN,SOME (propT --> preT) ,NoSyn)]
-  fun def_axioms ax_defs = (#2 o Specification.axiomatization ax_defs [] [] [])
-
   fun def_resF cmraT = (#2 o Typedecl.abbrev_global (resFN,["'a", "'b"],NoSyn) cmraT)
   fun def_inv preT = (#2 o Typedecl.abbrev_global (invN,[],NoSyn) (subst_aT preT invT))
   fun def_res cmraT = (#2 o Typedecl.abbrev_global (resN,[],NoSyn) cmraT)
@@ -152,25 +144,20 @@ ML \<open>
       thy |> Config.put_global quick_and_dirty true |> f |> Config.put_global quick_and_dirty qad 
     end
 
-  (* Axiomatize that pre_iprop is of class ofe. This will mark the command with a red background. *)
-  fun pre_inst thy = Class.instance_arity_cmd ([Binding.name_of pre_ipropN], [], "ofe") thy
-    |> Proof.global_skip_proof false |> Proof_Context.theory_of
   in
 
   fun mk_iprop cmras thy = 
-    let val (preT,thy') = mk_pre_iprop thy 
+    let 
       val cmras_raw = map (fn (cmra,name)=>{camera=cmra, name=name, getter=NONE, constructor=NONE}) cmras
-      val cmra_data = {number = length cmras+3, cameras = cmras_raw@fixed_cmras preT, cmraPT = NONE}
+      val cmra_data = {number = length cmras+3, cameras = cmras_raw@fixed_cmras pre_ipropT, cmraPT = NONE}
       val cmra_data = mk_getters cmra_data
       val cmra_data = mk_owns cmra_data
-      val cmraT = subst_aT preT base_cameraT |> mk_cmraT (mk_maps (map fst cmras))
-      val propT = mk_pred cmraT 
-      val axs = mk_axioms preT propT
+      val cmraT = subst_aT pre_ipropT base_cameraT |> mk_cmraT (mk_maps (map fst cmras))
       val cmra_data = {number = #number cmra_data, cameras = #cameras cmra_data, cmraPT = SOME cmraT}
-    in thy' |> 
+    in thy |> 
       wrap_quick_and_dirtys_mode (fn thy => thy
-        |> def_axioms axs |> def_resF cmraT |> def_inv preT |> def_res cmraT |> def_iprop cmraT
-        |> pre_inst |> Named_Target.theory_map (mk_defs cmra_data)
+        |> def_resF cmraT |> def_inv pre_ipropT |> def_res cmraT |> def_iprop cmraT
+        |> Named_Target.theory_map (mk_defs cmra_data)
       )
     end
 end;
@@ -181,13 +168,6 @@ type_synonym lockG = "unit ex"
 setup \<open>mk_iprop [(\<^typ>\<open>graphUR auth\<close>, "graph"), (\<^typ>\<open>markingUR auth\<close>, "markings"), 
   (\<^typ>\<open>heap_lang_proph_map\<close>, "proph"), (\<^typ>\<open>lockG\<close>, "lock")]\<close>
   
-lemma iprop_fp: "iProp (pre P) = P" sorry
-declare [[coercion iProp]]
-
-lemma n_equiv_pre [simp]: "n_equiv n (pre P) (pre Q) \<longleftrightarrow> n_equiv n P Q" sorry
-
-term "\<epsilon>::res"
-
 text \<open>Again some experiments wrt the iprop fixed-point\<close>
 definition inv_map :: "('a::cofe \<Rightarrow> 'b::cofe) \<Rightarrow> ('a pre_inv \<Rightarrow> 'b pre_inv)" where 
   "inv_map (f::'a\<Rightarrow>'b) = map_prod (map_map_view (map_later f)) id"
@@ -264,40 +244,34 @@ specification (isos)
   sorry
 
 text \<open>inG instance examples\<close>
-context begin
-interpretation idInG: inG "\<lambda>\<gamma> (m::gname \<rightharpoonup> 'a::camera). m \<gamma>" "\<lambda>\<gamma> x. [\<gamma>\<mapsto>x]"
-apply (auto simp: d_equiv inG_def prod_n_valid_def \<epsilon>_n_valid op_prod_def
-  \<epsilon>_left_id intro: non_expansiveI)
-by (auto simp: pcore_prod_def pcore_fun_def \<epsilon>_fun_def \<epsilon>_option_def pcore_option_def comp_def split: option.splits)
-  
+interpretation idInG: inG "\<lambda>\<gamma> (m::gname \<rightharpoonup> 'a::ucamera). m \<gamma>" "\<lambda>\<gamma> x. [\<gamma>\<mapsto>x]"
+apply (auto simp: inG_def prod_n_valid_def \<epsilon>_n_valid op_prod_def \<epsilon>_left_id)
+apply (auto simp: pcore_prod_def pcore_fun_def \<epsilon>_fun_def \<epsilon>_option_def pcore_option_def comp_def 
+  split: option.splits)
+using singleton_map_only_n_equiv by metis
+
+interpretation invInG: inG get_inv constr_inv
+  apply (auto simp: inG_def get_inv_def constr_inv_def dest!: singleton_map_only_n_equiv)
+  apply (auto simp: d_equiv n_equiv_fun_def n_equiv_option_def prod_n_valid_def \<epsilon>_n_valid op_prod_def \<epsilon>_left_id)
+  by (auto simp: pcore_prod_def pcore_fun_def \<epsilon>_fun_def \<epsilon>_option_def pcore_option_def comp_def 
+    constr_inv_def split: option.splits)
+
 global_interpretation lockInG: inG get_lock constr_lock
 apply (auto simp: get_lock_def constr_lock_def d_equiv inG_def prod_n_valid_def \<epsilon>_n_valid op_prod_def
-  \<epsilon>_left_id intro: non_expansiveI)
-by (auto simp: pcore_prod_def pcore_fun_def \<epsilon>_fun_def \<epsilon>_option_def pcore_option_def comp_def constr_lock_def split: option.splits)
+  \<epsilon>_left_id intro: map_upd_eqD1)
+by (auto simp: pcore_prod_def pcore_fun_def \<epsilon>_fun_def \<epsilon>_option_def pcore_option_def comp_def
+  constr_lock_def singleton_map_n_incl split: option.splits)
 
-interpretation graphInG: inG get_graph constr_graph
-apply (auto simp: get_graph_def constr_graph_def d_equiv inG_def prod_n_valid_def \<epsilon>_n_valid op_prod_def
-  \<epsilon>_left_id intro: non_expansiveI)
-by (auto simp: pcore_prod_def pcore_fun_def \<epsilon>_fun_def \<epsilon>_option_def pcore_option_def comp_def constr_graph_def split: option.splits)
+global_interpretation prophInG: inG get_proph constr_proph
+apply (auto simp: get_proph_def constr_proph_def d_equiv inG_def prod_n_valid_def \<epsilon>_n_valid op_prod_def
+  \<epsilon>_left_id intro: map_upd_eqD1)
+by (auto simp: pcore_prod_def pcore_fun_def \<epsilon>_fun_def \<epsilon>_option_def pcore_option_def comp_def
+  constr_proph_def singleton_map_n_incl split: option.splits)
 
+context begin
 private lemma testlemma: "inG (getter::gname\<Rightarrow>'a::ucamera\<Rightarrow>lockG option) put
   \<Longrightarrow> 1=2" sorry
   
 thm testlemma[OF lockInG.inG_axioms]
-
-context
-fixes getl :: "gname \<Rightarrow> 'a::ucamera \<Rightarrow> lockG option"
-  and putl
-  and getg :: "gname \<Rightarrow> 'a \<Rightarrow> graphUR auth option"
-  and putg
-assumes lock_in: "inG getl putl" 
-  and graph_in: "inG getg putg"
-begin
-  lemma testlemma2: False sorry
-  definition some_prop :: "'a upred_f" where "some_prop \<equiv> Own putl 0 (Ex ())"
-end
-
-thm testlemma2[OF lockInG.inG_axioms graphInG.inG_axioms]
-term "some_prop constr_lock"
 end
 end
