SpinLock/SpinLock.thy
@@ -11,14 +11,17 @@ definition acquire :: val where "acquire \<equiv>
 definition release :: val where "release \<equiv>
   V\<lambda> (Some ''l''): ((V ''l'') \<leftarrow> FalseE)"
 
+declare lockInG.inG_axioms[lock_inG_axiom, inG_axioms]
+  
 definition "lock_name :: gname \<equiv> 7"
 definition lockN :: namespace where "lockN \<equiv> add_name nroot (string_to_name ''spin_lock'')"
 
+context includes heap_syntax begin
 definition lock_inv :: "gname \<Rightarrow> loc \<Rightarrow> iprop \<Rightarrow> iprop" where
   "lock_inv \<gamma> l R \<equiv> \<exists>\<^sub>u b. l\<mapsto>\<^sub>u#[b] \<^emph> (\<upharpoonleft>b \<or>\<^sub>u (\<upharpoonleft>(\<not>b) \<^emph> (own constr_lock \<gamma> (Ex ())) \<^emph> R))"
 
 definition is_lock :: "gname \<Rightarrow> val \<Rightarrow> iprop \<Rightarrow> iprop" where
-  "is_lock \<gamma> lk R \<equiv> \<exists>\<^sub>u l. \<upharpoonleft>(lk=#[l]) \<and>\<^sub>u inv lockN (lock_inv \<gamma> l R)"
+  "is_lock \<gamma> lk R \<equiv> \<exists>\<^sub>u l. \<upharpoonleft>(lk=#[l]) \<and>\<^sub>u inv constr_inv lockN (lock_inv \<gamma> l R)"
 
 definition "locked \<gamma> \<equiv> own constr_lock \<gamma> (Ex ())"
 
@@ -46,7 +49,7 @@ lemma lock_alloc: "\<exists>\<^sub>u \<gamma>.\<Rrightarrow>\<^sub>b (locked \<g
   apply iIntro
   apply (iExistsR "0::nat")
   unfolding locked_def
-  apply (entails_substR rule: rule: lockInG.own_alloc)
+  apply (entails_substR rule:  lockInG.own_alloc)
   by (auto simp: valid_def constr_lock_def prod_n_valid_def \<epsilon>_n_valid valid_raw_ex_def)
 
 lemmas [iris_simp] = lock_inv_def locked_def is_lock_def newlock_def acquire_def release_def
@@ -54,37 +57,37 @@ lemmas [iris_simp] = lock_inv_def locked_def is_lock_def newlock_def acquire_def
 lemma newlock_spec:
   "{{ upred_emp }} App newlock #[()] {{ \<lambda>lk. \<forall>\<^sub>u R. (R ={UNIV}=\<^emph> (\<exists>\<^sub>u \<gamma>. is_lock \<gamma> lk R)) }}"
   \<comment> \<open>Unfold newlock definition\<close>
-  apply (auto simp: newlock_def subst'_def intro!: wp_pure[OF pure_exec_beta])
+  apply (auto simp: newlock_def subst'_def intro!: wp_pure[OF wp_inG pure_exec_beta])
   \<comment> \<open>Remove wp based on @{thm wp_alloc}.\<close>
-  apply (iApply rule: wp_alloc)
-  apply (iDestruct rule: wp_mono)
+  apply (iApply rule: wp_alloc[OF wp_inG])
+  apply (iDestruct rule: wp_mono[OF wp_inG])
   \<comment> \<open>Allocate lock and \<^const>\<open>lock_inv\<close>.\<close>
   apply (rule upred_forallI, rule upred_wandI)
   apply (rule add_holds[OF lock_alloc])
   apply iExistsL subgoal for v l R \<gamma>
-  apply (iMod rule: upd_fupd)
-  apply (iApply_step "?P" rule: inv_alloc[of "lock_inv _ _ R" _ lockN])
+  apply (iMod rule: upd_fupd[OF invInG.inG_axioms])
+  apply (iApply_step "?P" rule: inv_alloc[OF invInG.inG_axioms, of "lock_inv _ _ R" _ lockN])
   apply (entails_substR rule: upred_laterI)
   apply (iExistsR False)
   apply (iFrame2 "?l\<mapsto>\<^sub>uFalseV\<^emph>R")
   apply (rule upred_entails_refl)
   \<comment> \<open>Cleanup\<close>
-  apply (rule fupd_mono)
+  apply (rule fupd_mono[OF invInG.inG_axioms])
   by (iExistsR \<gamma>)
   oops
 
 (* Once again with another wp rule. Is more similar to the Coq version.*)
 lemma newlock_spec:
   "{{ upred_emp }} App newlock #[()] {{ \<lambda>lk. \<forall>\<^sub>u R. (R ={UNIV}=\<^emph> (\<exists>\<^sub>u \<gamma>. is_lock \<gamma> lk R)) }}"
-  apply (auto simp: newlock_def subst'_def intro!: wp_pure[OF pure_exec_beta])
+  apply (auto simp: newlock_def subst'_def intro!: wp_pure[OF wp_inG pure_exec_beta])
   apply (iWP rule: wp_alloc')
-  apply (entails_substR rule: wp_value)
+  apply (entails_substR rule: wp_value[OF wp_inG])
   apply iForallR
   apply (rule upred_wandI)
   apply (iDestruct rule: lock_alloc)
-  apply (iMod rule: upd_fupd)
+  apply (iMod rule: upd_fupd[OF invInG.inG_axioms])
   subgoal for l R \<gamma>
-  apply (iMod_step "?P" rule: inv_alloc[of "lock_inv _ _ R" _ lockN])
+  apply (iMod_step "?P" rule: inv_alloc[OF invInG.inG_axioms, of "lock_inv _ _ R" _ lockN])
   apply (entails_substR rule: upred_laterI)
   apply iExistsR2
   apply (iFrame2 "?l\<mapsto>\<^sub>u?b") by frame_single+
@@ -94,9 +97,9 @@ lemma release_spec:
   "{{ is_lock \<gamma> lk R \<^emph> locked \<gamma> \<^emph> R }} App release lk {{ \<lambda>_. upred_emp }}"  
   \<comment> \<open>Unfold release definition\<close>
   apply (simp add: release_def is_lock_def upred_pure_sep_conj' pull_exists_eq pull_exists_eq')
-  apply (iDestruct rule: wp_pure[OF pure_exec_beta]) subgoal for l
+  apply (iDestruct rule: wp_pure[OF wp_inG pure_exec_beta]) subgoal for l
   \<comment> \<open>Open invaraint\<close>
-  apply (iMod rule: inv_acc[OF subset_UNIV])
+  apply (iMod rule: inv_acc[OF invInG.inG_axioms subset_UNIV])
   \<comment> \<open>Apply @{thm wp_store}\<close>
   apply (move_sepL "\<triangleright> ?P")
   unfolding upred_later_exists
@@ -107,7 +110,7 @@ lemma release_spec:
   apply (iWP rule: wp_store')
   \<comment> \<open>Cleanup\<close>
   apply (entails_substR rule: upred_laterI)
-  apply (entails_substR rule: wp_value)
+  apply (entails_substR rule: wp_value[OF wp_inG])
   apply (iApply_wand_as_rule "\<exists>\<^sub>u (x::bool). ?P x" "(?l\<mapsto>\<^sub>u?v)\<^emph>(lockInG.own ?n ?x)\<^emph>R")
   apply (iExistsR False)
   apply (entails_substR rule: upred_laterI)
@@ -163,17 +166,17 @@ apply brute_force_solver
 oops
 end
   
-lemmas spinlock_intros[intro] = wp_store'[simplified] 
+lemmas spinlock_intros[intro] = wp_store'[OF wp_inG, simplified] 
   upred_entails_substE[OF upred_entail_eqL[OF upred_later_sep]]
-  wp_pure[OF pure_exec_beta] wp_alloc' upred_entails_trans[OF _ wp_value]
-  wp_mono upred_forallI upred_wandI upred_existsE'
-  upred_entails_substE[OF upd_fupd[to_entailment]] elim_modal_entails'[OF elim_modal_fupd]
+  wp_pure[OF wp_inG pure_exec_beta] wp_alloc'[OF wp_inG] upred_entails_trans[OF _ wp_value[OF wp_inG]]
+  wp_mono[OF wp_inG] upred_forallI upred_wandI upred_existsE'
+  upred_entails_substE[OF upd_fupd[OF invInG.inG_axioms, to_entailment]] elim_modal_entails'[OF elim_modal_fupd[OF invInG.inG_axioms]]
   elim_modal_entails[OF elim_modal_timeless'] elim_modal_entails'[OF elim_modal_timeless']
   upred_entails_trans[OF upred_wand_apply'] upred_entails_trans[OF _ upred_laterI] log_prog_rule
   upred_existsI upred_pure_impl upred_pure_impl' upred_pureI upred_pureI' upred_entails_refl 
   upred_weakeningR upred_weakeningL fupd_mono upred_entails_conjI  
   framing' can_be_split_refl can_be_split_baseR can_be_split_sepL
-  elim_modal_entails'[OF elim_modal_fupd_wp_atomic]
+  elim_modal_entails'[OF elim_modal_fupd_wp_atomic] wp_inG
     
 lemma move_pure: "(\<upharpoonleft>b) \<^emph> P = P \<^emph> \<upharpoonleft>b" "P \<^emph> (\<upharpoonleft>b) \<^emph> Q = P \<^emph> Q \<^emph> (\<upharpoonleft>b)"
     apply (rule upred_sep_comm) by (rule upred_sep_comm2_eq)
@@ -189,9 +192,10 @@ definition diaframe_hint :: "iprop \<Rightarrow> ('b \<Rightarrow> iprop) \<Righ
 lemma hintE: "diaframe_hint H L M A U \<Longrightarrow> (\<And>y::'b. (H \<^emph> L y \<turnstile> M (\<exists>\<^sub>u x::'a. A x \<^emph> U y x)))"
   unfolding diaframe_hint_def by simp
   
-lemma inv_hint: "diaframe_hint upred_emp (\<lambda>x::'a. \<triangleright>(L x)) (linear_fupd E) (\<lambda>x::'a. inv N (L x)) (\<lambda>_ x::'a. inv N (L x))"
+lemma inv_hint: "diaframe_hint upred_emp (\<lambda>x::'a. \<triangleright>(L x)) (linear_fupd E) 
+  (\<lambda>x::'a. inv constr_inv N (L x)) (\<lambda>_ x::'a. inv constr_inv N (L x))"
   apply (auto simp: diaframe_hint_def)
-  apply (iMod rule: inv_alloc[to_entailment])
+  apply (iMod rule: inv_alloc[OF invInG.inG_axioms, to_entailment])
   apply iExistsR2
   apply (rule upred_entails_trans[OF upred_entail_eqR[OF persistent_dupl]])
   by auto
@@ -199,11 +203,11 @@ lemma inv_hint: "diaframe_hint upred_emp (\<lambda>x::'a. \<triangleright>(L x))
 lemma biabd_hint_apply_aux: 
   assumes "diaframe_hint H L (fancy_upd E3 E2) A U"
   shows "H \<^emph> \<Turnstile>{E1,E3}=> (\<exists>\<^sub>u y. L y \<^emph> (\<forall>\<^sub>u x. (U y x) -\<^emph> (G x))) \<turnstile> \<Turnstile>{E1,E2}=> (\<exists>\<^sub>u x. G x \<^emph> A x)"
-  apply (entails_substR rule: fupd_mask_trans[of _ E3])
-  apply (iMod rule: fupd_frame_r[where ?R=H])
+  apply (entails_substR rule: fupd_mask_trans[OF invInG.inG_axioms, of _ E3])
+  apply (iMod rule: fupd_frame_r[OF invInG.inG_axioms, where ?R=H])
   apply iExistsL
   apply (iApply rule: hintE[OF assms])
-  apply (iMod rule: fupd_frame_r[where ?R="(\<forall>\<^sub>ux. U _ x -\<^emph> G x)"])
+  apply (iMod rule: fupd_frame_r[OF invInG.inG_axioms, where ?R="(\<forall>\<^sub>ux. U _ x -\<^emph> G x)"])
   apply iExistsL subgoal for y x
   apply (iExistsR x)
   apply (rule pull_forall_antecedent')
@@ -236,14 +240,14 @@ lemma wp_store_hint:"diaframe_hint upred_emp (\<lambda>_. \<Turnstile>{UNIV,E}=>
   (linear_fupd UNIV) (\<lambda>_. WP (Store #[l] (Val v)) {{ \<Phi> }}) (\<lambda>_ _. upred_emp)"
   unfolding diaframe_hint_def
   apply (simp add: drop_exists)
-  apply(entails_substR rule: fupd_intro)
-  apply (rule elim_modal_entails[OF elim_modal_fupd_wp_atomic[OF atomic_store]])
+  apply(entails_substR rule: fupd_intro[OF invInG.inG_axioms])
+  apply (rule elim_modal_entails[OF elim_modal_fupd_wp_atomic[OF wp_inG atomic_store]])
   apply iExistsL
   apply (move_sepL "\<triangleright>(?l\<mapsto>\<^sub>u?v)")
   apply later_elim
-  apply (rule wp_store'[unfolded to_val_simp])
+  apply (rule wp_store'[OF wp_inG, unfolded to_val_simp])
   apply (rule upred_later_mono_extL)
-  apply (rule upred_entails_trans[OF _ wp_value])
+  apply (rule upred_entails_trans[OF _ wp_value[OF wp_inG]])
   by iApply_wand
   
 lemmas inv_alloc' = biabd_hint_apply[OF inv_hint]
@@ -258,7 +262,9 @@ lemma newlock_spec:
   apply (rule add_holds[OF lock_alloc])
   apply (simp | step)+
   apply (rule inv_alloc'[where ?G = "\<lambda> _. upred_emp",simplified])
-  apply (entails_substR rule: fupd_intro[to_entailment])
+  apply (entails_substR rule: fupd_intro[OF invInG.inG_axioms, to_entailment])
+  apply (simp | step)
+  apply (simp | step)
   apply (simp | step)
   apply (simp | step)
   apply (simp | step)
@@ -278,10 +284,11 @@ ML \<open>
   val f = Term.could_beta_contract x
 \<close>
 
-lemma move_invR: "inv N Q \<^emph> P = P \<^emph> inv N Q" "P \<^emph> inv N R \<^emph> Q = P \<^emph> Q \<^emph> inv N R"
+lemma move_invR: "inv constr_inv N Q \<^emph> P = P \<^emph> inv constr_inv N Q" 
+  "P \<^emph> inv constr_inv N R \<^emph> Q = P \<^emph> Q \<^emph> inv constr_inv N R"
   apply (rule upred_sep_comm) by (rule upred_sep_comm2_eq)
 
-lemma move_invL: "P \<^emph> inv N Q = inv N Q \<^emph> P" by (rule upred_sep_comm)
+lemma move_invL: "P \<^emph> inv constr_inv N Q = inv constr_inv N Q \<^emph> P" by (rule upred_sep_comm)
 
 lemma move_closerL: "P \<^emph> (Q={UNIV - names N,UNIV}=\<^emph>upred_emp) = (Q={UNIV - names N,UNIV}=\<^emph>upred_emp) \<^emph> P"
   by (rule upred_sep_comm)
@@ -295,8 +302,8 @@ method inv_opener =
   (rule upred_entails_substE[OF upred_entail_eqR[OF persistent_dupl]]
   | rule upred_entails_substE'[OF upred_entail_eqR[OF persistent_dupl]]),
   fast, unfold upred_sep_assoc_eq,
-  (rule upred_entails_substE[OF inv_acc[to_entailment,OF subset_UNIV]]
-  | rule upred_entails_substE'[OF inv_acc[to_entailment,OF subset_UNIV]]),
+  (rule upred_entails_substE[OF inv_acc[OF invInG.inG_axioms, to_entailment,OF subset_UNIV]]
+  | rule upred_entails_substE'[OF inv_acc[OF invInG.inG_axioms, to_entailment,OF subset_UNIV]]),
   (unfold move_closerL)?
 
 lemma release_spec: 
@@ -322,7 +329,7 @@ lemma release_spec:
 declare spinlock_intros[rule del]
 declare new_lock_simps[simp del]
 
-declare frame_rule_apply[OF upred_entails_trans[OF upred_entails_trans[OF lock_alloc[to_entailment] upred_exist_mono[OF upd_fupd[to_entailment]], unfolded locked_def] fupd_exists_lift], alloc_rule]
+declare frame_rule_apply[OF upred_entails_trans[OF upred_entails_trans[OF lock_alloc[to_entailment] upred_exist_mono[OF upd_fupd[to_entailment]], unfolded locked_def] fupd_exists_lift[OF invInG.inG_axioms]], alloc_rule]
 declare upred_later_exists[iris_simp]
 declare upred_entails_trans[OF store_hint[where ?G = upred_emp, unfolded emp_rule to_val_simp] fupd_wp, wp_symbolic_execution_steps]
 declare frame_baseL[frame_rule]
@@ -334,4 +341,5 @@ lemma newlock_spec:
 lemma release_spec: 
   "{{{ is_lock \<gamma> lk R \<^emph> locked \<gamma> \<^emph> R }}} App release lk {{{ \<lambda>_. upred_emp }}}"
   by brute_force_solver
+end
 end
